external/Goose/github_com/mit_pdos/gokv/simplepb/state.v
@@ -32,16 +32,18 @@ Definition Clerk__FetchAndAppend: val :=
 
 Definition KVState := struct.decl [
   "kvs" :: mapT (slice.T byteT);
-  "filename" :: stringT;
   "epoch" :: uint64T;
-  "nextIndex" :: uint64T
+  "nextIndex" :: uint64T;
+  "sealed" :: boolT;
+  "filename" :: stringT
 ].
 
 Definition Op: ty := slice.T byteT.
 
-Definition KVState__loadState: val :=
-  rec: "KVState__loadState" "s" "snap_in" :=
-    (* log.Println("Loading encoded state: ", len(snap_in)) *)
+(* helper for unmarshalling kvs *)
+Definition KVState__decodeKvs: val :=
+  rec: "KVState__decodeKvs" "s" "snap_in" :=
+    (* log.Println("Decoding encoded state of length: ", len(snap_in)) *)
     let: "snap" := ref_to (slice.T byteT) "snap_in" in
     struct.storeF KVState "kvs" "s" (NewMap (slice.T byteT) #());;
     let: ("numEntries", "snap") := marshal.ReadInt (![slice.T byteT] "snap") in
@@ -62,6 +64,16 @@ Definition KVState__loadState: val :=
       Continue);;
     #().
 
+Definition KVState__encodeKvs: val :=
+  rec: "KVState__encodeKvs" "s" :=
+    let: "enc" := ref_to (slice.T byteT) (NewSlice byteT #0) in
+    "enc" <-[slice.T byteT] marshal.WriteInt (![slice.T byteT] "enc") (MapLen (struct.loadF KVState "kvs" "s"));;
+    MapIter (struct.loadF KVState "kvs" "s") (λ: "k" "v",
+      "enc" <-[slice.T byteT] marshal.WriteInt (![slice.T byteT] "enc") "k";;
+      "enc" <-[slice.T byteT] marshal.WriteInt (![slice.T byteT] "enc") (slice.len "v");;
+      "enc" <-[slice.T byteT] marshal.WriteBytes (![slice.T byteT] "enc") "v");;
+    ![slice.T byteT] "enc".
+
 Definition RecoverKVState: val :=
   rec: "RecoverKVState" "fname" :=
     let: "s" := struct.alloc KVState (zero_val (struct.t KVState)) in
@@ -71,6 +83,7 @@ Definition RecoverKVState: val :=
     then
       struct.storeF KVState "epoch" "s" #0;;
       struct.storeF KVState "nextIndex" "s" #0;;
+      struct.storeF KVState "sealed" "s" #false;;
       struct.storeF KVState "kvs" "s" (NewMap (slice.T byteT) #())
     else
       let: ("0_ret", "1_ret") := marshal.ReadInt (![slice.T byteT] "encState") in
@@ -79,28 +92,21 @@ Definition RecoverKVState: val :=
       let: ("0_ret", "1_ret") := marshal.ReadInt (![slice.T byteT] "encState") in
       struct.storeF KVState "nextIndex" "s" "0_ret";;
       "encState" <-[slice.T byteT] "1_ret";;
-      KVState__loadState "s" (![slice.T byteT] "encState"));;
+      KVState__decodeKvs "s" (![slice.T byteT] "encState"));;
     "s".
 
-Definition KVState__GetState: val :=
-  rec: "KVState__GetState" "s" :=
+Definition KVState__getState: val :=
+  rec: "KVState__getState" "s" :=
     let: "enc" := ref_to (slice.T byteT) (NewSlice byteT #0) in
-    "enc" <-[slice.T byteT] marshal.WriteInt (![slice.T byteT] "enc") (MapLen (struct.loadF KVState "kvs" "s"));;
-    MapIter (struct.loadF KVState "kvs" "s") (λ: "k" "v",
-      "enc" <-[slice.T byteT] marshal.WriteInt (![slice.T byteT] "enc") "k";;
-      "enc" <-[slice.T byteT] marshal.WriteInt (![slice.T byteT] "enc") (slice.len "v");;
-      "enc" <-[slice.T byteT] marshal.WriteBytes (![slice.T byteT] "enc") "v");;
+    "enc" <-[slice.T byteT] marshal.WriteInt (![slice.T byteT] "enc") (struct.loadF KVState "epoch" "s");;
+    "enc" <-[slice.T byteT] marshal.WriteInt (![slice.T byteT] "enc") (struct.loadF KVState "nextIndex" "s");;
+    "enc" <-[slice.T byteT] marshal.WriteBytes (![slice.T byteT] "enc") (KVState__encodeKvs "s");;
     (* log.Println("Size of encoded state", len(enc)) *)
     ![slice.T byteT] "enc".
 
 Definition KVState__MakeDurable: val :=
   rec: "KVState__MakeDurable" "s" :=
-    let: "state" := KVState__GetState "s" in
-    let: "enc" := ref_to (slice.T byteT) (NewSliceWithCap byteT #0 (#16 + slice.len "state")) in
-    "enc" <-[slice.T byteT] marshal.WriteInt (![slice.T byteT] "enc") (struct.loadF KVState "epoch" "s");;
-    "enc" <-[slice.T byteT] marshal.WriteInt (![slice.T byteT] "enc") (struct.loadF KVState "nextIndex" "s");;
-    "enc" <-[slice.T byteT] marshal.WriteBytes (![slice.T byteT] "enc") "state";;
-    grove_ffi.Write (struct.loadF KVState "filename" "s") (![slice.T byteT] "enc");;
+    grove_ffi.Write (struct.loadF KVState "filename" "s") (KVState__getState "s");;
     #().
 
 Definition KVState__Apply: val :=
@@ -113,10 +119,19 @@ Definition KVState__Apply: val :=
     "ret".
 
 Definition KVState__SetState: val :=
-  rec: "KVState__SetState" "s" "snap_in" :=
-    KVState__loadState "s" "snap_in";;
+  rec: "KVState__SetState" "s" "snap_in" "epoch" "nextIndex" :=
+    KVState__decodeKvs "s" "snap_in";;
+    struct.storeF KVState "epoch" "s" "epoch";;
+    struct.storeF KVState "nextIndex" "s" "nextIndex";;
     KVState__MakeDurable "s";;
     #().
+
+Definition KVState__GetStateAndSeal: val :=
+  rec: "KVState__GetStateAndSeal" "s" :=
+    let: "ret" := KVState__encodeKvs "s" in
+    struct.storeF KVState "sealed" "s" #true;;
+    KVState__MakeDurable "s";;
+    "ret".
 
 Definition KVState__EnterEpoch: val :=
   rec: "KVState__EnterEpoch" "s" "epoch" :=
@@ -129,8 +144,7 @@ Definition MakeKVStateMachine: val :=
     struct.new pb.StateMachine [
       "Apply" ::= KVState__Apply "initState";
       "SetState" ::= KVState__SetState "initState";
-      "GetState" ::= KVState__GetState "initState";
-      "EnterEpoch" ::= KVState__EnterEpoch "initState"
+      "GetStateAndSeal" ::= KVState__GetStateAndSeal "initState"
     ].
 
 Definition KVServer := struct.decl [
